Weidenbach_Book/IsaSAT_Conflict_Analysis.thy
@@ -265,44 +265,6 @@ lemma tl_state_wl_heur_tl_state_wl:
 definition (in -) get_max_lvl_st :: \<open>nat twl_st_wl \<Rightarrow> nat literal \<Rightarrow> nat\<close> where
   \<open>get_max_lvl_st S L = get_maximum_level_remove (get_trail_wl S) (the (get_conflict_wl S)) L\<close>
 
-definition (in -) lookup_conflict_remove1 :: \<open>nat literal \<Rightarrow> lookup_clause_rel \<Rightarrow> lookup_clause_rel\<close> where
-  \<open>lookup_conflict_remove1 =
-     (\<lambda>L (n,xs). (n-1, xs [atm_of L := NOTIN]))\<close>
-
-lemma lookup_conflict_remove1:
-  \<open>(uncurry (RETURN oo lookup_conflict_remove1), uncurry (RETURN oo remove1_mset))
-   \<in> [\<lambda>(L,C). L \<in># C \<and> -L \<notin># C \<and> L \<in> snd ` D\<^sub>0]\<^sub>f
-     Id \<times>\<^sub>f lookup_clause_rel \<rightarrow> \<langle>lookup_clause_rel\<rangle>nres_rel\<close>
-  apply (intro frefI nres_relI)
-  apply (case_tac y; case_tac x)
-  subgoal for x y a b aa ab c
-    using mset_as_position_remove[of c b \<open>atm_of aa\<close>]
-    by (cases \<open>aa\<close>)
-      (auto simp: lookup_clause_rel_def lookup_conflict_remove1_def lookup_clause_rel_atm_in_iff
-        minus_notin_trivial2 size_remove1_mset_If in_\<L>\<^sub>a\<^sub>l\<^sub>l_atm_of_in_atms_of_iff minus_notin_trivial
-        mset_as_position_in_iff_nth)
-   done
-
-definition (in -) lookup_conflict_remove1_pre :: \<open>nat literal \<times> nat \<times> bool option list \<Rightarrow> bool\<close> where
-\<open>lookup_conflict_remove1_pre = (\<lambda>(L,(n,xs)). n > 0 \<and> atm_of L < length xs)\<close>
-
-sepref_thm conflict_remove1_code
-  is \<open>uncurry (RETURN oo lookup_conflict_remove1)\<close>
-  :: \<open>[lookup_conflict_remove1_pre]\<^sub>a unat_lit_assn\<^sup>k *\<^sub>a lookup_clause_rel_assn\<^sup>d \<rightarrow>
-     lookup_clause_rel_assn\<close>
-  supply [[goals_limit=2]] one_uint32_nat[sepref_fr_rules]
-  unfolding lookup_conflict_remove1_def one_uint32_nat_def[symmetric] fast_minus_def[symmetric]
-  lookup_conflict_remove1_pre_def
-  by sepref
-
-concrete_definition (in -) conflict_remove1_code
-  uses isasat_input_bounded_nempty.conflict_remove1_code.refine_raw
-  is \<open>(uncurry ?f,_)\<in>_\<close>
-
-prepare_code_thms (in -) conflict_remove1_code_def
-
-lemmas conflict_remove1_code_refine[sepref_fr_rules] =
-   conflict_remove1_code.refine[of \<A>\<^sub>i\<^sub>n, OF isasat_input_bounded_nempty_axioms]
 
 definition (in isasat_input_ops) update_confl_tl_wl_heur
   :: \<open>nat \<Rightarrow> nat literal \<Rightarrow> twl_st_wl_heur \<Rightarrow> (bool \<times> twl_st_wl_heur) nres\<close>
